examples/dev/sw/ARMCompositionScript.sml
@@ -19,20 +19,6 @@ val _ = Globals.priming := NONE;
 (* Additional theorems for finite maps                                                                  *)
 (*------------------------------------------------------------------------------------------------------*)
 
-(* Sort in ascending order *)
-val FUPDATE_LT_COMMUTES = Q.store_thm (
-  "FUPDATE_LT_COMMUTES",
-  ` !f a b c d. c < a ==> (f |+ (a:num, b) |+ (c,d) = f |+ (c,d) |+ (a,b))`,
-    RW_TAC arith_ss [FUPDATE_COMMUTES]
-    );
-
-(* Sort in descending order                                                                             *)
-val FUPDATE_GT_COMMUTES = Q.store_thm (
-  "FUPDATE_GT_COMMUTES",
-  ` !f a b c d. c > a ==> (f |+ (a:ADDR,b) |+ (c,d) = f |+ (c,d) |+ (a,b))`,
-    RW_TAC arith_ss [FUPDATE_COMMUTES]
-    );
-
 
 val fupdate_normalizer =
  let val thm = SPEC_ALL FUPDATE_LT_COMMUTES
